---
date: 2024-07-19
tags:
  - an-introduction-to-manifolds
---
# Smooth vs. Analytic Functions

We denote the coordinates on $\R^n$ as $x^1,\dots,x^n$ and a point $p=(p^1,\dots,p^n)$.

> [!def] 
> A real-valued function $f:U\rightarrow\R$ is said to be $C^k$ at $p\in U$ if its partial derivatives
> $$
> 	\frac{\partial^j f}{\partial x^{i_1}\cdots\partial x^{i_j}}
> $$
> of all orders $j\le k$ exist and are continuous at $p$. It is $C^\infty$ or **smooth** if it is $C^k$ for all $k\ge0$.

Some examples include:
1. Polynomials are $C^\infty$ over $\R$
2. The function $f:\R\rightarrow\R$ given by $f(x)=x^{1/3}$ is $C^0$ but not $C^1$ at $x=0$.
3. The function $g:\R\rightarrow\R$ given by $g(x)=\frac{3}{4}x^{4/3}$ has derivative $g'(x)=f(x)=x^{1/3}$, so $g$ is $C^1$ but not $C^2$ at $x=0$.

We define a **neighborhood** of a point in $\R^n$ to be an open set containing the point. A function $f$ is **real-analytic** at $p$ if in a neighborhood of $p$ it is equal to it's Taylor series at $p$:
$$
	f(x) = f(p) + \sum_{i}\frac{\partial f}{\partial x^i}(p)(x^i-p^i) + \frac{1}{2!}\sum_{i,j}\frac{\partial^2f}{\partial x^i\partial x^j}(p)(x^i-p^i)(x^j-p^j) + \dots.
$$
All real-analytic functions are necessarily $C^\infty$ because the convergent power series can be differentiated. For example, if 
$$
	f(x)=\sin x=x-\frac{1}{3!}x^3+\frac{1}{5!}x^5-\cdots
$$
then we can differentiate to get
$$
	f'(x)=\cos x=1-\frac{1}{2!}x^2 + \frac{1}{4!}x^4 - \cdots
$$
However, not all $C^\infty$ functions are real-analytic. For example consider the function
$$
	f(x) = \begin{cases}
		e^{-1/x} & \text{if }x>0 \\
		0 & \text{if }x\le 0.
	\end{cases}
$$
Notice that for $x>0$
$$
\begin{align*}
	f'(x) &= \frac{e^{-1/x}}{x^2} \\
	f''(x) &= \frac{e^{-1/x}(1-2x)}{x^4} \\
	f'''(x) &= \frac{e^{-1/x}(6x^2-6x+1)}{x^6} \\
	&\vdots \\
	f^{(k)}(x) &= e^{-1/x}p_{2k}(1/x)~\text{ for some polynomial }p_{2k}\text{ of degree }2k.
\end{align*}
$$
Thus, if we let $x\rightarrow0$, (making use of L'Hopital's rule)
$$
\begin{align*}
	\lim_{x\rightarrow0}e^{-1/x}p_{2k}(1/x) &= \lim_{x\rightarrow0}\frac{p_{2k}(1/x)}{e^{1/x}} \\
	&= \lim_{x\rightarrow0}\frac{p_{2k-1}(1/x)}{e^{1/x}} \\
	&\phantom{=}\vdots \\
	&= \lim_{x\rightarrow0}\frac{0}{e^{1/x}} = 0.
\end{align*}
$$
Hence, $f^{(k)}=0$ for all $k\ge0$. Therefore, $f$ is $C^\infty$ but the Taylor series at the origin is zero in every neighborhood, i.e., $f$ is not real-analytic.

# Taylor's Theorem with Remainder

We say a subset $S\subset\R^n$ is **star-shaped** with respect to $p\in S$ if for every $x\in S$, the line segment from $p$ to $x$ lies in $S$. For example:

![[Screenshot from 2024-07-19 13-11-54.png#invert | center]]

The set $S$ is star-shaped with respect to $p$, but not $q$.

> [!lemma] Taylor's theorem with remainder
> Let $f$ be a $C^\infty$ function on an open subset $U$ of $\R^n$ star-shaped with respect to a point $p=(p^1,\dots,p^n)$ in $U$. Then there are functions $g_1(x),\dots,g_n(x)\in C^\infty(U)$ such that 
> $$
> 	f(x) = f(p) + \sum_{i=1}^n(x^i-p^i)g_i(x),~ g_i(p) = \frac{\partial f}{\partial x^i}(p).
> $$

**Proof:**
Notice that for any $x\in U$ the line segment $p+t(x-p)$, $0\le t\le 1$ lies in $U$ since $U$ is star-shaped with respect to $p$. If we differentiate using the chain rule
$$
	\frac{d}{dt}f(p+t(x-p)) = \sum(x^i-p^i)\frac{\partial f}{\partial x^i}(p+t(x-p)).
$$
If we integrate both sides from 0 to 1,
$$
	f(p+t(x-p))\Big|_0^1 = \sum(x^i-p^i)\int_0^1\frac{\partial f}{\partial x^i}(p+t(x-p))dt.
$$
Letting 
$$
	g_i(x) = \int_0^1\frac{\partial f}{\partial x^i}(p+t(x-p))
$$
gives the result.

# Problems

##### 1.3. A diffeomorphism of an open interval with $\R$
Let $U\subset\R^n$ and $V\subset\R^n$ be open intervals. A $C^\infty$ map $F:U\rightarrow V$ is called a **diffeomorphism** if it is bijective and has a $C^\infty$ inverse $F^{-1}:V\rightarrow U$. Show that any two finite intervals are diffeomorphic.

**Answer:** Let $a<b$ and define $f:(0,1)\rightarrow(a,b)$ by $f(t)=ta+(1-t)b$. Notice that $f$ is $C^\infty(0,1)$ since 
$$
\begin{align*}
	f'(t) &= a - b \\
	f''(t) &= 0
\end{align*}
$$
are continuous. Moreover, $f$ is bijective with inverse
$$
	f^{-1}(x) = \frac{x-b}{a-b}
$$
and 
$$
	\frac{d}{dx}f^{-1}(x) = \frac{1}{a-b}\text{ and }\frac{d^2}{dx^2}f^{-1}(x) = 0.
$$
Therefore, $f$ is a diffeomorphism. Since $a$ and $b$ are arbitrary, it follows that all finite intervals $(a,b)$ are diffeomorphic.

##### 1.5. A diffeomorphism of an open ball with $\R^n$
Let $\textbf{0}=(0,0)$ be the origin and $B(\textbf{0},1)$ be the open unit disk in $\R^2$. To find a diffeomorphism between $B(\textbf{0},1)$ and $\R^2$, we identify $\R^2$ with the $xy$-plane in $\R^3$ and introduce the lower open hemisphere
$$
	S: x^2+y^2+(z-1)^2 = 1,~z < 1,
$$
in $\R^3$ as an intermediate space. Note that the map
$$
	f:B(\textbf{0},1)\rightarrow S,~(a,b)\mapsto(a,b,1-\sqrt{1-a^2-b^2})
$$
is a bijection.

(a) The *stereographic projection* $g:S\rightarrow\R^2$ from $(0,0,1)$ is the map that sends a point $(a,b,c)\in S$ to the intersection of the line through $(0,0,1)$ and $(a,b,c)$ with the $xy$-plane. Determine the map $g$ and it's inverse.

![[Screenshot from 2024-07-19 14-11-06.png#invert | center]]


**Answer:** We seek the map $(a,b,c)\mapsto(u,v)$ for $(a,b,c)\in S$. By similar triangles (working in the $xz$-plane), notice that 
$$
	\frac{u-a}{c} = \frac{u}{1}.
$$
Solving for $u$ we get that $u=a/(1-c)$. We repeat this in the $yz$-plane to get $v=b/(1-c)$. Therefore, $g$ is given by
$$
	(a,b,c)\mapsto \left(\frac{a}{1-c},\frac{b}{1-c}\right).	
$$
We now seek the inverse map $g^{-1}$. Notice that $(a,b,c)\in S$ implies that $c=1-\sqrt{1-a^2-b^2}$. Hence, solving for $a$ and $b$ gives us
$$
	(u,v)\mapsto\left(\frac{u}{\sqrt{1+u^2+v^2}},\frac{v}{\sqrt{1+u^2+v^2}},1-\frac{1}{\sqrt{1+u^2+v^2}}\right).
$$

(b) Composing the two maps $f$ and $g$ gives the map
$$
	h=g\circ f:B(\textbf{0},1)\rightarrow\R^2,~h(a,b)=\left(\frac{a}{\sqrt{1-a^2-b^2}},\frac{b}{\sqrt{1-a^2-b^2}}\right).
$$
Find the formula for $h^{-1}(u,v)$ and conclude that $h$ is a diffeomorphism of the open disk $B(\textbf{0},1)$ with $\R^2$.

**Answer:** Notice that 
$$
\begin{align*}
	h^{-1}(u,v) &= (f^{-1}\circ g^{-1})(u,v) \\
	&= f^{-1}\left(\frac{u}{\sqrt{1+u^2+v^2}},\frac{v}{\sqrt{1+u^2+v^2}},1-\frac{1}{\sqrt{1+u^2+v^2}}\right) \\
	&= \left(\frac{u}{\sqrt{1+u^2+v^2}},\frac{v}{\sqrt{1+u^2+v^2}}\right)
\end{align*}
$$
One may verify that $h$ and $h^{-1}$ are $C^\infty$.

