---
date: 2024-08-02
---
The **cotangent space** at $p\in\R^n$, denoted $T_p^*(\R^n)$, is the dual of the tangent space, i.e., $(T_p\R^n)^\vee$. Hence, a cotangent $f\in T_p^*(\R^n)$ is a linear functional $f:T_p(\R^n)\rightarrow\R$. 

A **covector field** or a **differential 1-form** (1-form for short) on an open subset $U\subset\R^n$ is a map $\omega$ that assigns to each point $p\in U$ a covector
$$
\begin{align*}
	\omega:U\rightarrow\bigcup_{p\in U}T_p^*(\R^n) \\
	p\mapsto\omega_p\in T_p^*(\R^n).
\end{align*}
$$
From any $C^\infty$ function $f:U\rightarrow\R$ we can construct a 1-form $df$ called the **differential** of $f$: for $p\in U$ and $X_p\in T_pU$ we define
$$
	(df)_p(X_p) = X_pf = \sum a^i(p)\frac{\partial f}{\partial x^i}.
$$
Recall that $\{\partial/\partial x^1|_p,\dots,\partial/\partial x^n|_p\}$ is a basis for the tangent space $T_p(\R^n)$.

> [!prp] 
> If $x^1,\dots,x^n$ are the standard coordinates on $\R^n$, then at each $p\in\R^n$, $\{(dx^1)_p,\dots,(dx^n)_p\}$ is the basis for the cotangent space $T_p^*(\R^n)$.

**Proof:** Notice that
$$
	(dx^i)_p\left(\frac{\partial}{\partial x^j}\Bigg|_p\right) = \frac{\partial}{\partial x^j}\Bigg|_px^i = \delta_j^i.
$$
<p style='text-align: right'>Q.E.D.</p>

Thus, we can represent $\omega\in T_p^*(\R^n)$ by the linear combination
$$
	\omega_p = \sum a_i(p)(dx^i)_p
$$
for some $a_i(p)\in\R$. 

> [!prp] 
> If $f:U\rightarrow\R$ is a $C^\infty$ function on an open set $U$ in $\R^n$ then
> $$
> 	df = \sum\frac{\partial f}{\partial x^i}dx^i.
> $$

**Proof:** From proposition 4.1, $df=\sum a_idx^i$ for some functions $a_i:U\rightarrow\R$. Notice that
$$
	\frac{\partial f}{\partial x^j} = df\left(\frac{\partial}{\partial x^j}\right) = \sum a^idx^i\left(\frac{\partial}{\partial x^j}\right) = \sum a
	_i\delta_j^i = a_j.
$$
<p style='text-align: right'>Q.E.D.</p>

# Differential k-Forms

A **differential form of degree k** or **k-form** $\omega$ on an open subset $U$ of $\R^n$ is a function that assigns to each point $p\in U$ an alternating $k$-linear function on the tangent space, i.e., $p\mapsto\omega_p\in A_k(T_p\R^n)$. Note that $A_1(T_p\R^n)=T_p^*(\R^n$).

Recall that a basis for $A_k(T_p\R^n)$ is
$$
	dx_p^I = dx_p^{i_1}\wedge\cdots\wedge dx_p^{i_k},~1\le i_1<\cdots<i_k\le n.
$$
Therefore, at each point $p\in U$, $\omega_p$ is the linear combination
$$
	\omega_p = \sum a_I(p)dx_p^I
$$
so
$$
	\omega = \sum a_Idx^I
$$
with function coefficients $a_I:U\rightarrow\R$. We say a $k$-form is $C^\infty$ on $U$ if each coefficient $a_I$ is $C^\infty$ on $U$. We denote the vector space of $C^\infty$ $k$-forms on $U$ by $\Omega^k(U)$.

Let $\omega$ be a $k$-form and $\tau$ an $\ell$-form on $U$. Then we define the **wedge product** of $\omega$ and $\tau$ to be $(k+\ell)$-form defined pointwise:
$$
	(\omega\wedge\tau)_p = \omega_p\wedge\tau_p.
$$
In terms of coordinates, if $\omega=\sum a_Idx^I$ and $\tau=\sum b_Jdx^J$, then
$$
	\omega\wedge\tau = \sum_{I,J} (a_Ib_J)dx^I\wedge dx^J = \sum_{I,J\text{ disjoint}}(a_Ib_J)dx^I\wedge dx^J.
$$
One may show that the wedge product is anticommutative and associative.

Note that a zero form maps a point $p\in U$ to an element of $A_0(T_p\R^n)$, an alternating 0-linear function, i.e., a constant function. Thus, a 0-form is simply a function $\omega:U\rightarrow\R$. Notice then that if $f\in\Omega^0(U)$ and $\omega\in \Omega^k(U)$, then $f\wedge\omega$ is the $k$-form defined by pointwise multiplication
$$
	(f\wedge\omega)_p = f_p\wedge\omega_p = f(p)\omega_p,
$$
i.e., $f\wedge\omega=f\omega$.

**Example:** Let $x,y,z$ be the coordinates for $\R^3$. The $C^\infty$ 1-forms on $\R^3$ are of the form
$$
	fdx + gdy + hdz
$$
where $f,g,h:\R^3\rightarrow\R$ are $C^\infty$ functions. The $C^\infty$ 2-forms are
$$
	fdy\wedge dz + gdx\wedge dz + hdx\wedge dy
$$
and the $C^\infty$ 3-forms are
$$
	fdx\wedge dy\wedge dz.
$$
There are no non-zero $k$-forms for $k>3$.

# Differential Forms as Multilinear Functions on Vector Fields

Let $\omega$ be a $C^\infty$ 1-form and $X$ a $C^\infty$ vector field on $U\subset\R^n$. We define $\omega(X)$ on $U$ by
$$
	\omega(X)_p = \omega_p(X_p)
$$
or if $\omega=\sum a_idx^i$ and $X=\sum b^j\frac{\partial}{\partial x^j}$, then
$$
	w(X) = \left(\sum a_idx^i\right)\left(\sum b^j\frac{\partial}{\partial x^j}\right) = \sum a_ib^i.
$$
Thus, a $C^\infty$ 1-form gives rise to map between vector fields $\mathfrak{X}(U)$ to smooth functions $C^\infty(U)$. This function is linear over the ring $C^\infty(U)$, i.e., if $f\in C^\infty(U)$ then
$$
	\omega(fX) = f\omega(X).
$$
Indeed, let $p\in U$ and notice that
$$
\begin{align*}
	(\omega(fX))_p &= \omega_p(f(p)X_p) = f(p)\omega_p(X_p) = (f\omega(X))_p.
\end{align*}
$$
Thus a 1-form $\omega$ on $U$ gives rise to an $C^\infty(U)$-linear map $\mathfrak{X}(U)\rightarrow C^\infty(U)$ given by $X\mapsto\omega(X)$. Likewise, a $k$-form $\omega$ gives rise to a $k$-linear map
$$
\begin{align*}
	\mathfrak{X}(U)\times\cdots\times\mathfrak{X}(U)\rightarrow C^\infty(U) \\\
	(X_1,\dots,X_k)\mapsto\omega(X_1,\dots,X_k).
\end{align*}
$$

# The Exterior Derivative

Let $f:U\rightarrow\R$ be $C^\infty$. We define the exterior derivative of $f$ to be the differential $df\in\Omega^1(U)$ given by
$$
	df = \sum\frac{\partial f}{\partial x^i}dx^i.
$$
We then can use this definition to define the exterior derivative of a $k$-form.

> [!def]
> For $k\ge 1$, if $\omega=\sum_I a_Idx^I\in\Omega^k(U)$, then the **exterior derivative** is given by
> $$
> 	d\omega = \sum_Ida_I\wedge dx^I = \sum_I\left(\sum_j\frac{\partial a_I}{\partial x^j}dx^j\right)\wedge dx^I\in\Omega^{k+1}(U).
> $$

**Example:** Consider the 1-form $fdx+gdy$ on $\R^2$, where $f,g:\R^2\rightarrow\R$ are $C^\infty$. Then
$$
\begin{align*}
	d\omega &= df\wedge dx + dg\wedge dy \\
	&= \left(\frac{\partial f}{\partial x}dx + \frac{\partial f}{\partial y}dy\right)\wedge dx + \left(\frac{\partial g}{\partial x}dx + \frac{\partial g}{\partial y}dy\right)\wedge dy \\
	&= \frac{\partial f}{\partial x}dx\wedge dx + \frac{\partial f}{\partial y}dy\wedge dx + \frac{\partial g}{\partial x}dx\wedge dy+\frac{\partial g}{\partial y}dy\wedge dy \\
	&= \left(\frac{\partial g}{\partial x}-\frac{\partial f}{\partial y}\right)dx\wedge dy.
\end{align*}
$$

> [!def]
> Let $A=\bigoplus_{k=0}^\infty A^k$ be a graded algebra over a field $K$. An **antiderivation** of a graded algebra $A$ is a $K$-linear map $D:A\rightarrow A$ such that for $a\in A^k$ and $b\in A^\ell$,
> $$
> 	D(ab) = (Da)b + (-1)^kaDb.
> $$
> If $D$ sends $A^k$ to $A^{k+m}$ for all $k$, then we say that has **degree** $m$.

> [!prp]
> 1. The **exterior differentiation** $d:\Omega^*(U)\rightarrow\Omega^*(U)$ is an antiderivation of degree 1:
> $$
> 	d(\omega\wedge\tau) = (d\omega)\wedge\tau + (-1)^{\textup{deg}\omega}\omega\wedge d\tau
> $$
> 2. $d^2=0$
> 3. If $f\in C^\infty(U)$ and $X\in\mathfrak{X}(U)$, then $(df)(X) = Xf$.

**Proof:**
1. Let $\omega=fdx^I$ and $\tau=g dx^J$. Notice that 
$$
\begin{align*}
	d(\omega\wedge\tau) &= d(fgdx^I\wedge dx^J) \\
	&= \sum\frac{\partial fg}{\partial x^i}dx^i\wedge dx^I\wedge dx^J \\
	&= \sum\frac{\partial f}{\partial x^i}gdx^i\wedge dx^I\wedge dx^J + \sum f\frac{\partial g}{\partial x^i}dx^i\wedge dx^I\wedge dx^J \\
	&= \sum\frac{\partial f}{\partial x^i}dx^i\wedge dx^I\wedge gdx^J + (-1)^k\sum fdx^I\wedge \frac{\partial g}{\partial x^i}dx^i\wedge dx^J \\
	&= d\omega\wedge\tau + (-1)^k\omega\wedge d\tau.
\end{align*}
$$
The rest follows by linearity.

2. Let $\omega=fdx^I$. Notice that
$$
\begin{align*}
	d^2\omega &= d\left(\sum\frac{\partial f}{\partial x^i}dx^i\wedge dx^I\right) = \sum\frac{\partial^2f}{\partial x^j\partial x^i}dx^j\wedge dx^i\wedge dx^I.
\end{align*}
$$
In the sum, when $i=j$ we get $dx^j\wedge dx^i=0$. For $i\ne j$, the two symmetric terms cancel
$$
\frac{\partial^2}{\partial x^i\partial x^j}dx^i\wedge dx^j + \frac{\partial^2}{\partial x^j\partial x^i}dx^j\wedge dx^i = \frac{\partial^2f}{\partial x^i\partial x^j}dx^i\wedge dx^j+\frac{\partial^2f}{\partial x^i\partial x^j}(-dx^i\wedge dx^j) = 0.
$$
Therefore, $d^2\omega=0$.

3. Notice that for $X=\sum b^j\frac{\partial}{\partial x^j}$,
$$
	(df)(X) = \left(\sum\frac{\partial f}{\partial x^i}dx^i\right)(X) = \sum\frac{\partial f}{\partial x^i}b^i = Xf.
$$
<p style='text-align: right'>Q.E.D.</p>
> [!prp]
> If $D:\Omega^*(U)\rightarrow\Omega^*(U)$ satisfies properties (1)-(3) in the previous proposition, then $D=d$.

# Closed Forms and Exact Forms

A $k$-form on $U$ is **closed** if $d\omega=0$; it is **exact** if there is a $(k-1)$-form $\tau$ such that $\omega=d\tau$ on $U$. Since $d^2=0$, every exact form is closed.

**Example:** Define the 1-form $\omega$ on $\R^2\setminus\{0\}$ by
$$
	\omega=\frac{1}{x^2+y^2}(-ydx + xdy).
$$
Notice that
$$
\begin{align*}
	d\omega &= \left(\frac{2xy}{(x^2+y^2)^2}dx+\frac{y^2-x^2}{(x^2+y^2)^2}dy\right)\wedge dx + \left(\frac{y^2-x^2}{(x^2+y^2)^2}dx-\frac{2xy}{(x^2+y^2)^2}dy\right)\wedge dy \\
	&= \frac{y^2-x^2}{(x^2+y^2)^2}dy\wedge dx + \frac{y^2-x^2}{(x^2+y^2)^2}dx\wedge dy \\
	&= -\frac{y^2-x^2}{(x^2+y^2)^2}dx\wedge dy + \frac{y^2-x^2}{(x^2+y^2)^2}dx\wedge dy \\
	&= 0.
\end{align*}
$$
Therefore, $\omega$ is exact.

For any open subset $U\subset\R^n$, the exterior derivative $d$ forms a differential complex called the **de Rham complex** of $U$ given by
$$
	0\rightarrow\Omega^0(U)\rightarrow\Omega^1(U)\rightarrow\Omega^2(U)\rightarrow\cdots.
$$
The closed forms are in the kernel of $d$, and the exact forms are in the image of $d$.

# Applications to Vector Calculus

A **vector-valued** function is a function $\textbf{F}:\langle P,Q,R\rangle:U\rightarrow\R^3$ that assigns to each point $p\in U$ a vector $F_p\in\R^3\cong T_p(\R^3)$. Hence, a vector-valued function on $U$ is a vector field on $U$. Recall that
$$
\begin{align*}
	\textup{grad}~f &= \nabla\cdot f = \langle\frac{\partial f}{\partial x},\frac{\partial f}{\partial y},\frac{\partial f}{\partial z}\rangle, \\
	\textup{curl}~\textbf{F} &= \nabla\times\textbf{F} = \langle\frac{\partial F_z}{\partial y}-\frac{\partial F_y}{\partial z}, \frac{\partial F_x}{\partial z}-\frac{\partial F_z}{\partial x}, \frac{\partial F_y}{\partial x}-\frac{\partial F_x}{\partial y}\rangle \\
	\textup{div}~\textbf{F} &= \nabla\cdot\textbf{F} = \frac{\partial F_x}{\partial x} + \frac{\partial F_y}{\partial y} + \frac{\partial F_z}{\partial z}.
\end{align*}
$$
Since a 1-form on $U$ is a linear combination of $dx$, $dy$, $dz$, we can identify 1-forms via vectors
$$
	Pdx + Qdy + Rdz \longleftrightarrow \langle P,Q,R\rangle
$$
and 2-forms
$$
	Pdy\wedge dz + Qdz\wedge dx + Rdx\wedge dy \longleftrightarrow\langle P,Q,R\rangle
$$
and 3-forms
$$
	fdx\wedge dy\wedge dz \longleftrightarrow f.
$$
In this form, we can see that
$$
\begin{align*}
	df &\longleftrightarrow \textup{grad}~f \\
	d(Pdx + Qdy + Rdz) &\longleftrightarrow \textup{curl}\langle P,Q,R\rangle \\
	d(Pdy\wedge dz + Qdz\wedge dx + Rdx\wedge dy) &\longleftrightarrow \textup{div}\langle P,Q,R\rangle.
\end{align*}
$$
In other words, the gradient is the exterior derivative on a 0-form. The curl is the exterior derivative on a 1-form, and the divergence is the exterior derivative on a 2-form. Or, in visual terms:

![[Screenshot from 2024-08-02 16-27-16.png#invert | center]]

From this identification, we easy get the following proposition.

> [!prp]
> 1. $\textup{curl}(\textup{grad}~f)=0$
> 2. $\textup{div}(\textup{curl}~f)=0$
> 3. On $\R^3$, a vector field $\textbf{F}$ is the gradient of some scalar $f$ if and only if $\textup{curl}~\textbf{F}=0$.

**Proof:** Properties 1 and 2 follow from the property $d^2=0$. Property 3 is due to the fact that a 1-form on $\R^3$ is exact if and only if it is closed.
<p style='text-align: right'>Q.E.D.</p>
Note that property 3 may not hold on a region other than $\R^3$.

**Example:** If $U=\R^3\setminus\{z\text{-axis}\}$ and
$$
	\textbf{F} = \langle\frac{-y}{x^2+y^2},\frac{x}{x^2+y^2},0\rangle
$$
on $\R^3$, then $\textup{curl}~\textbf{F}=0$, but $\textbf{F}$ is not the gradient of any $C^\infty$ function on $U$. Assume it was. Then by the fundamental theorem of Calculus for line integrals
$$
	\int_C-\frac{y}{x^2+y^2}dx+\frac{x}{x^2+y^2}dy = 0
$$
for any closed curve $C$. However, on the unit circle with $x=\cos t$ and $y=\sin t$ we get
$$
	\int_C-\frac{y}{x^2+y^2}dx+\frac{x}{x^2+y^2}dy = \int_0^{2\pi}-(\sin t)d\cos t+(\cos t)d\sin t = \int_0^{2\pi}dt = 2\pi.
$$
A contradiction.